finish spec of one implementation

theories/coneris/examples/random_counter.v
@@ -4,114 +4,178 @@ From clutch.coneris Require Import coneris hocap.
 
 Set Default Proof Using "Type*".
 
-(* Class lock `{!conerisGS Σ} := Lock *)
-(* { *)
-(*   (** * Operations *) *)
-(*   new_counter : val; *)
-(*   incr_counter : val; *)
-(*   allocate_tape : val; *)
-(*   incr_counter_tape : val; *)
-(*   (** * Ghost state *) *)
-(*   (** The assumptions about [Σ] *) *)
-(*   counterG : gFunctors → Type; *)
-(*   (** [name] is used to associate [locked] with [is_lock] *) *)
-(*   error_name : Type; *)
-(*   tape_name: Type; *)
-(*   counter_name: Type; *)
-(*   (** * Predicates *) *)
-(*   is_counter {L : counterG Σ} (N:namespace) (counter: val) *)
-(*     (γ1: error_name) (γ2: tape_name) (γ3: counter_name): iProp Σ; *)
-(*   counter_error_auth {L : counterG Σ} (γ: error_name) (x:R): iProp Σ; *)
-(*   counter_error_frag {L : counterG Σ} (γ: error_name) (x:R): iProp Σ; *)
-(*   counter_tapes_auth {L : counterG Σ} (γ: tape_name) (m:gmap loc (nat*list nat)): iProp Σ; *)
-(*   counter_tapes_frag {L : counterG Σ} (γ: tape_name) (α:loc) (N:nat) (ns:list nat): iProp Σ; *)
-(*   counter_content_auth {L : counterG Σ} (γ: counter_name) (z:Z): iProp Σ; *)
-(*   counter_content_frag {L : counterG Σ} (γ: counter_name) (f:frac) (z:Z): iProp Σ; *)
-(*   (** * General properties of the predicates *) *)
-(*   #[global] is_counter_persistent {L : counterG Σ} N c γ1 γ2 γ3 :: *)
-(*     Persistent (is_counter (L:=L) N c γ1 γ2 γ3); *)
-(*   #[global] counter_error_auth_timeless {L : counterG Σ} γ x :: *)
-(*     Timeless (counter_error_auth (L:=L) γ x); *)
-(*   #[global] counter_error_frag_timeless {L : counterG Σ} γ x :: *)
-(*     Timeless (counter_error_frag (L:=L) γ x); *)
-(*   #[global] counter_tapes_auth_timeless {L : counterG Σ} γ m :: *)
-(*     Timeless (counter_tapes_auth (L:=L) γ m); *)
-(*   #[global] counter_tapes_frag_timeless {L : counterG Σ} γ α N ns :: *)
-(*     Timeless (counter_tapes_frag (L:=L) γ α N ns); *)
-(*   #[global] counter_content_auth_timeless {L : counterG Σ} γ z :: *)
-(*     Timeless (counter_content_auth (L:=L) γ z); *)
-(*   #[global] counter_content_frag_timeless {L : counterG Σ} γ f z :: *)
-(*     Timeless (counter_content_frag (L:=L) γ f z); *)
+Class random_counter `{!conerisGS Σ} := RandCounter
+{
+  (** * Operations *)
+  new_counter : val;
+  incr_counter : val;
+  allocate_tape : val;
+  incr_counter_tape : val;
+  read_counter : val;
+  (** * Ghost state *)
+  (** The assumptions about [Σ] *)
+  counterG : gFunctors → Type;
+  (** [name] is used to associate [locked] with [is_lock] *)
+  error_name : Type;
+  tape_name: Type;
+  counter_name: Type;
+  (** * Predicates *)
+  is_counter {L : counterG Σ} (N:namespace) (counter: val)
+    (γ1: error_name) (γ2: tape_name) (γ3: counter_name): iProp Σ;
+  counter_error_auth {L : counterG Σ} (γ: error_name) (x:R): iProp Σ;
+  counter_error_frag {L : counterG Σ} (γ: error_name) (x:R): iProp Σ;
+  counter_tapes_auth {L : counterG Σ} (γ: tape_name) (m:gmap loc (nat*list nat)): iProp Σ;
+  counter_tapes_frag {L : counterG Σ} (γ: tape_name) (α:loc) (N:nat) (ns:list nat): iProp Σ;
+  counter_content_auth {L : counterG Σ} (γ: counter_name) (z:nat): iProp Σ;
+  counter_content_frag {L : counterG Σ} (γ: counter_name) (f:frac) (z:nat): iProp Σ;
+  (** * General properties of the predicates *)
+  #[global] is_counter_persistent {L : counterG Σ} N c γ1 γ2 γ3 ::
+    Persistent (is_counter (L:=L) N c γ1 γ2 γ3);
+  #[global] counter_error_auth_timeless {L : counterG Σ} γ x ::
+    Timeless (counter_error_auth (L:=L) γ x);
+  #[global] counter_error_frag_timeless {L : counterG Σ} γ x ::
+    Timeless (counter_error_frag (L:=L) γ x);
+  #[global] counter_tapes_auth_timeless {L : counterG Σ} γ m ::
+    Timeless (counter_tapes_auth (L:=L) γ m);
+  #[global] counter_tapes_frag_timeless {L : counterG Σ} γ α N ns ::
+    Timeless (counter_tapes_frag (L:=L) γ α N ns);
+  #[global] counter_content_auth_timeless {L : counterG Σ} γ z ::
+    Timeless (counter_content_auth (L:=L) γ z);
+  #[global] counter_content_frag_timeless {L : counterG Σ} γ f z ::
+    Timeless (counter_content_frag (L:=L) γ f z);
 
-(*   counter_error_auth_exclusive {L : counterG Σ} γ x1 x2: *)
-(*     counter_error_auth (L:=L) γ x1 -∗ counter_error_auth (L:=L) γ x2 -∗ False;  *)
-(*   counter_error_frag_exclusive {L : counterG Σ} γ x1 x2: *)
-(*   counter_error_frag (L:=L) γ x1 -∗ counter_error_frag (L:=L) γ x2 -∗ False; *)
-(*   counter_error_agree {L : counterG Σ} γ x1 x2: *)
-(*     counter_error_auth (L:=L) γ x1 -∗ counter_error_frag (L:=L) γ x2 -∗ ⌜x1 = x2 ⌝;  *)
-(*   counter_error_update {L : counterG Σ} γ x1 x2 x3: *)
-(*     counter_error_auth (L:=L) γ x1 -∗ counter_error_frag (L:=L) γ x2 ==∗ *)
-(*     counter_error_auth (L:=L) γ x3 ∗ counter_error_frag (L:=L) γ x3; *)
+  counter_error_auth_exclusive {L : counterG Σ} γ x1 x2:
+    counter_error_auth (L:=L) γ x1 -∗ counter_error_auth (L:=L) γ x2 -∗ False;
+  counter_error_frag_exclusive {L : counterG Σ} γ x1 x2:
+  counter_error_frag (L:=L) γ x1 -∗ counter_error_frag (L:=L) γ x2 -∗ False;
+  counter_error_agree {L : counterG Σ} γ x1 x2:
+    counter_error_auth (L:=L) γ x1 -∗ counter_error_frag (L:=L) γ x2 -∗ ⌜x1 = x2 ⌝;
+  counter_error_update {L : counterG Σ} γ x1 x2 (x3:nonnegreal):
+    counter_error_auth (L:=L) γ x1 -∗ counter_error_frag (L:=L) γ x2 ==∗
+    counter_error_auth (L:=L) γ x3 ∗ counter_error_frag (L:=L) γ x3;
 
-(*   counter_tapes_auth_exclusive {L : counterG Σ} γ m1 m2: *)
-(*     counter_tapes_auth (L:=L) γ m1 -∗ counter_tapes_auth (L:=L) γ m2 -∗ False;  *)
-(*   counter_tapes_frag_exclusive {L : counterG Σ} γ α N N' ns ns': *)
-(*   counter_tapes_frag (L:=L) γ α N ns -∗ counter_tapes_frag (L:=L) γ α N' ns' -∗ False; *)
-(*   counter_tapes_agree {L : counterG Σ} γ α m N ns: *)
-(*     counter_tapes_auth (L:=L) γ m -∗ counter_tapes_frag (L:=L) γ α N ns -∗ ⌜ m!! α = Some (N, ns) ⌝;  *)
-(*   counter_tapes_update {L : counterG Σ} γ α m N ns n: *)
-(*     counter_tapes_auth (L:=L) γ m -∗ counter_tapes_frag (L:=L) γ α N ns ==∗ *)
-(*     counter_tapes_auth (L:=L) γ (<[α := (N, ns ++[n])]> m) ∗ counter_tapes_frag (L:=L) γ α N (ns ++ [n]); *)
+  (* counter_tapes_auth_exclusive {L : counterG Σ} γ m m': *)
+  (* counter_tapes_auth (L:=L) γ m -∗ counter_tapes_auth (L:=L) γ m' -∗ False; *)
+  counter_tapes_frag_exclusive {L : counterG Σ} γ α N N' ns ns':
+  counter_tapes_frag (L:=L) γ α N ns -∗ counter_tapes_frag (L:=L) γ α N' ns' -∗ False;
+  counter_tapes_agree {L : counterG Σ} γ α m N ns:
+    counter_tapes_auth (L:=L) γ m -∗ counter_tapes_frag (L:=L) γ α N ns -∗ ⌜ m!! α = Some (N, ns) ⌝;
+  counter_tapes_update {L : counterG Σ} γ α m N ns n:
+    counter_tapes_auth (L:=L) γ m -∗ counter_tapes_frag (L:=L) γ α N ns ==∗
+    counter_tapes_auth (L:=L) γ (<[α := (N, ns ++[n])]> m) ∗ counter_tapes_frag (L:=L) γ α N (ns ++ [n]);
 
-(*   counter_content_auth_exclusive {L : counterG Σ} γ z1 z2: *)
-(*     counter_content_auth (L:=L) γ z1 -∗ counter_content_auth (L:=L) γ z2 -∗ False;  *)
-(*   counter_content_less_than {L : counterG Σ} γ z z' f: *)
-(*     counter_content_auth (L:=L) γ z -∗ counter_content_frag (L:=L) γ f z' -∗ ⌜(z'<=z)%Z ⌝;  *)
-(*   counter_content_agree {L : counterG Σ} γ z z': *)
-(*     counter_content_auth (L:=L) γ z -∗ counter_content_frag (L:=L) γ 1%Qp z' -∗ ⌜(z'<=z)%Z ⌝; *)
-(*   counter_content_update {L : counterG Σ} γ f z1 z2 z3: *)
-(*     counter_content_auth (L:=L) γ z1 -∗ counter_content_frag (L:=L) γ f z2 ==∗ *)
-(*     counter_content_auth (L:=L) γ (z1+z3)%Z ∗ counter_content_frag (L:=L) γ f (z2+z3)%Z; *)
+  counter_content_auth_exclusive {L : counterG Σ} γ z1 z2:
+    counter_content_auth (L:=L) γ z1 -∗ counter_content_auth (L:=L) γ z2 -∗ False;
+  counter_content_less_than {L : counterG Σ} γ z z' f:
+    counter_content_auth (L:=L) γ z -∗ counter_content_frag (L:=L) γ f z' -∗ ⌜(z'<=z)%nat ⌝;
+  counter_content_agree {L : counterG Σ} γ z z':
+    counter_content_auth (L:=L) γ z -∗ counter_content_frag (L:=L) γ 1%Qp z' -∗ ⌜(z'=z)%nat ⌝;
+  counter_content_update {L : counterG Σ} γ f z1 z2 z3:
+    counter_content_auth (L:=L) γ z1 -∗ counter_content_frag (L:=L) γ f z2 ==∗
+    counter_content_auth (L:=L) γ (z1+z3)%nat ∗ counter_content_frag (L:=L) γ f (z2+z3)%nat;
   
-(*   (** * Program specs *) *)
-(*   new_counter_spec {L : counterG Σ} N ε: *)
-(*   {{{ ↯ ε }}} new_counter #() *)
-(*     {{{ c, RET c; ∃ γ1 γ2 γ3, is_counter (L:=L) N c γ1 γ2 γ3 ∗ *)
-(*                               counter_error_frag (L:=L) γ1 ε ∗ *)
-(*                               counter_content_frag (L:=L) γ3 1%Qp 0%Z *)
-(*     }}}; *)
-(*   (* acquire_spec `{!conerisGS Σ} {L : lockG Σ} γ lk R : *) *)
-(*   (*   {{{ is_lock (L:=L) γ lk R }}} acquire lk {{{ RET #(); locked (L:=L) γ ∗ R }}}; *) *)
-(*   (* release_spec `{!conerisGS Σ} {L : lockG Σ} γ lk R : *) *)
-(*   (*   {{{ is_lock (L:=L) γ lk R ∗ locked (L:=L) γ ∗ R }}} release lk {{{ RET #(); True }}} *) *)
-(* }. *)
+  (** * Program specs *)
+  new_counter_spec {L : counterG Σ} E ε N:
+  {{{ ↯ ε }}} new_counter #() @E
+    {{{ c, RET c; ∃ γ1 γ2 γ3, is_counter (L:=L) N c γ1 γ2 γ3 ∗
+                              counter_error_frag (L:=L) γ1 ε ∗
+                              counter_content_frag (L:=L) γ3 1%Qp 0%nat
+    }}};
+  incr_counter_spec {L: counterG Σ} E N c γ1 γ2 γ3 (ε2:R -> nat -> R) (P: iProp Σ) (T: nat -> iProp Σ) (Q: nat->nat->iProp Σ):
+    ↑N ⊆ E->
+    (∀ ε n, 0<= ε -> 0<= ε2 ε n)%R->
+    (∀ (ε:R), 0<=ε -> ((ε2 ε 0%nat) + (ε2 ε 1%nat)+ (ε2 ε 2%nat)+ (ε2 ε 3%nat))/4 <= ε)%R →
+    {{{ is_counter (L:=L) N c γ1 γ2 γ3 ∗
+        □(∀ (ε:R) (n : nat), P ∗ counter_error_auth (L:=L) γ1 ε ={E∖↑N}=∗ (⌜(1<=ε2 ε n)%R⌝∨ counter_error_auth (L:=L) γ1 (ε2 ε n) ∗ T n) ) ∗
+        □ (∀ (n:nat) (z:nat), T n ∗ counter_content_auth (L:=L) γ3 z ={E∖↑N}=∗
+                          counter_content_auth (L:=L) γ3 (z+n)%nat∗ Q z n) ∗
+        P
+    }}}
+      incr_counter c @ E
+      {{{ (n:nat) (z:nat), RET (#z, #n); Q z n }}};
+  allocate_tape_spec {L: counterG Σ} N E c γ1 γ2 γ3:
+    ↑N ⊆ E->
+    {{{ is_counter (L:=L) N c γ1 γ2 γ3 }}}
+      allocate_tape #() @ E
+      {{{ (v:val), RET v;
+          ∃ (α:loc), ⌜v=#lbl:α⌝ ∗ counter_tapes_frag (L:=L) γ2 α 3%nat []
+      }}};
+  incr_counter_tape_spec_some {L: counterG Σ} N E c γ1 γ2 γ3 (ε2:R -> nat -> R) (P: iProp Σ) (Q:nat->iProp Σ) (α:loc) (n:nat) ns:
+    ↑N⊆E -> 
+    {{{ is_counter (L:=L) N c γ1 γ2 γ3 ∗
+        □ (∀ (z:nat), P ∗ counter_content_auth (L:=L) γ3 z ={E∖↑N}=∗
+                          counter_content_auth (L:=L) γ3 (z+n)%nat ∗ Q z) ∗
+        P ∗ counter_tapes_frag (L:=L) γ2 α 3%nat (n::ns)
+    }}}
+      incr_counter_tape c #lbl:α @ E
+                                 {{{ (z:nat), RET (#z, #n); Q z ∗ counter_tapes_frag (L:=L) γ2 α 3%nat ns}}};
+  incr_counter_tape_spec_none {L: counterG Σ} N E c γ1 γ2 γ3 (ε2:R -> nat -> R) (P: iProp Σ) (T: nat -> iProp Σ) (Q: nat -> nat -> iProp Σ)(α:loc) (ns:list nat):
+    ↑N ⊆ E->
+    (∀ ε n, 0<= ε -> 0<= ε2 ε n)%R->
+    (∀ (ε:R), 0<=ε -> ((ε2 ε 0%nat) + (ε2 ε 1%nat)+ (ε2 ε 2%nat)+ (ε2 ε 3%nat))/4 <= ε)%R →
+    {{{ is_counter (L:=L) N c γ1 γ2 γ3 ∗
+        □(∀ (ε:R) (n : nat), P ∗ counter_error_auth (L:=L) γ1 ε
+                           ={E∖↑N}=∗ (⌜(1<=ε2 ε n)%R⌝∨ counter_error_auth (L:=L) γ1 (ε2 ε n) ∗ T n) ) ∗
+        □ (∀ (n:nat) (z:nat), T n ∗ counter_content_auth (L:=L) γ3 z  ={E∖↑N}=∗
+                          counter_content_auth (L:=L) γ3 (z+n)%nat ∗ Q z n) ∗
+        P ∗ counter_tapes_frag (L:=L) γ2 α 3%nat []
+    }}}
+      incr_counter_tape c #lbl:α @ E
+                                 {{{ (z:nat) (n:nat), RET (#z, #n); Q z n ∗ counter_tapes_frag (L:=L) γ2 α 3%nat [] }}};
+  counter_presample_spec {L: counterG Σ} NS (N : nat)  z E ns α
+     (ε2 : R -> nat -> R)
+    (P : iProp Σ) (Q : val-> iProp Σ) T γ1 γ2 γ3 c:
+    TCEq N (Z.to_nat z) →
+    ↑NS ⊆ E ->
+    (∀ ε n, 0<= ε -> 0<=ε2 ε n)%R ->
+    (∀ (ε:R), 0<= ε ->SeriesC (λ n, if (bool_decide (n≤N)) then 1 / (S N) * ε2 ε n else 0%R)%R <= ε)%R->
+    is_counter (L:=L) NS c γ1 γ2 γ3 -∗
+    (□∀ (ε:R) n, (P ∗ counter_error_auth (L:=L) γ1 ε) ={E∖↑NS}=∗
+        (⌜(1<=ε2 ε n)%R⌝ ∨ (counter_error_auth (L:=L) γ1 (ε2 ε n)  ∗ T (n)))) 
+        -∗
+    P -∗ counter_tapes_frag (L:=L) γ2 α N ns-∗
+        wp_update E (∃ n, T (n) ∗ counter_tapes_frag (L:=L) γ2 α N (ns++[n]));
+  read_counter_spec {L: counterG Σ} N E c γ1 γ2 γ3 P Q:
+    ↑N ⊆ E ->
+    {{{  is_counter (L:=L) N c γ1 γ2 γ3  ∗
+        □ (∀ (z:nat), P ∗ counter_content_auth (L:=L) γ3 z ={E∖↑N}=∗
+                    counter_content_auth (L:=L) γ3 z∗ Q z)
+         ∗ P
+    }}}
+      read_counter c @ E
+      {{{ (n':nat), RET #n'; Q n'
+      }}}
+}.
 
 
 Section impl1.
 
-  Definition new_counter : val:= λ: "_", ref #0.
-  Definition incr_counter : val := λ: "l", let: "n" := rand #3 in (FAA "l" "n", "n").
-  Definition allocate_tape : val := λ: "_", AllocTape #3.
-  Definition incr_counter_tape :val := λ: "l" "α", let: "n" := rand("α") #3 in (FAA "l" "n", "n").
-  Definition read_counter : val := λ: "l", !"l".
-
-  Context `{!conerisGS Σ, !hocap_errorGS Σ, !hocap_tapesGS Σ, !inG Σ (frac_authR ZR)}.
-  Definition counter_inv_pred (c:val) γ1 γ2 γ3:=
-    (∃ (ε:R) m (l:loc) (z:Z),
+  Definition new_counter1 : val:= λ: "_", ref #0.
+  Definition incr_counter1 : val := λ: "l", let: "n" := rand #3 in (FAA "l" "n", "n").
+  Definition allocate_tape1 : val := λ: "_", AllocTape #3.
+  Definition incr_counter_tape1 :val := λ: "l" "α", let: "n" := rand("α") #3 in (FAA "l" "n", "n").
+  Definition read_counter1 : val := λ: "l", !"l".
+  Class counterG1 Σ := CounterG1 { counterG1_error::hocap_errorGS Σ;
+                                   counterG1_tapes:: hocap_tapesGS Σ;
+                                   counterG1_frac_authR:: inG Σ (frac_authR natR) }.
+  
+  Context `{!conerisGS Σ, !hocap_errorGS Σ, !hocap_tapesGS Σ, !inG Σ (frac_authR natR)}.
+  Definition counter_inv_pred1 (c:val) γ1 γ2 γ3:=
+    (∃ (ε:R) m (l:loc) (z:nat),
         ↯ ε ∗ ●↯ ε @ γ1 ∗
         ([∗ map] α ↦ t ∈ m, α ↪N ( t.1 ; t.2 )) ∗ ●m@γ2 ∗  
         ⌜c=#l⌝ ∗ l ↦ #z ∗ own γ3 (●F z)
     )%I.
 
-  Lemma new_counter_spec E ε N:
+  Lemma new_counter_spec1 E ε N:
     {{{ ↯ ε }}}
-      new_counter #() @ E
+      new_counter1 #() @ E
       {{{ (c:val), RET c;
-          ∃ γ1 γ2 γ3, inv N (counter_inv_pred c γ1 γ2 γ3) ∗
-                      ◯↯ε @ γ1 ∗ own γ3 (◯F 0%Z)
+          ∃ γ1 γ2 γ3, inv N (counter_inv_pred1 c γ1 γ2 γ3) ∗
+                      ◯↯ε @ γ1 ∗ own γ3 (◯F 0%nat)
       }}}.
   Proof.
-    rewrite /new_counter.
+    rewrite /new_counter1.
     iIntros (Φ) "Hε HΦ".
     wp_pures.
     wp_alloc l as "Hl".
@@ -120,29 +184,30 @@ Section impl1.
     { lra. }
     simpl.
     iMod (hocap_tapes_alloc (∅:gmap _ _)) as "[%γ2 [H3 H4]]".
-    iMod (own_alloc (●F 0%Z ⋅ ◯F 0%Z)) as "[%γ3[H5 H6]]".
+    iMod (own_alloc (●F 0%nat ⋅ ◯F 0%nat)) as "[%γ3[H5 H6]]".
     { by apply frac_auth_valid. }
-    iMod (inv_alloc N _ (counter_inv_pred (#l) γ1 γ2 γ3) with "[$Hε $Hl $H1 $H3 $H5]") as "#Hinv".
+    replace (#0) with (#0%nat) by done.
+    iMod (inv_alloc N _ (counter_inv_pred1 (#l) γ1 γ2 γ3) with "[$Hε $Hl $H1 $H3 $H5]") as "#Hinv".
     { iSplit; last done. by iApply big_sepM_empty. }
     iApply "HΦ".
     iExists _, _, _. by iFrame.
   Qed. 
 
-  Lemma incr_counter_spec E N c γ1 γ2 γ3 (ε2:R -> nat -> R) (P: iProp Σ) (T: nat -> iProp Σ) (Q: Z->nat->iProp Σ):
+  Lemma incr_counter_spec1 E N c γ1 γ2 γ3 (ε2:R -> nat -> R) (P: iProp Σ) (T: nat -> iProp Σ) (Q: nat->nat->iProp Σ):
     ↑N ⊆ E->
     (∀ ε n, 0<= ε -> 0<= ε2 ε n)%R->
     (∀ (ε:R), 0<=ε -> ((ε2 ε 0%nat) + (ε2 ε 1%nat)+ (ε2 ε 2%nat)+ (ε2 ε 3%nat))/4 <= ε)%R →
-    {{{ inv N (counter_inv_pred c γ1 γ2 γ3) ∗
+    {{{ inv N (counter_inv_pred1 c γ1 γ2 γ3) ∗
         □(∀ (ε:R) (n : nat), P ∗ ●↯ ε @ γ1 ={E∖↑N}=∗ (⌜(1<=ε2 ε n)%R⌝∨●↯ (ε2 ε n) @ γ1 ∗ T n) ) ∗
-        □ (∀ (n:nat) (z:Z), T n ∗ own γ3 (●F z) ={E∖↑N}=∗
-                          own γ3 (●F(z+n)%Z)∗ Q z n) ∗
+        □ (∀ (n z:nat), T n ∗ own γ3 (●F z) ={E∖↑N}=∗
+                          own γ3 (●F(z+n)%nat)∗ Q z n) ∗
         P
     }}}
-      incr_counter c @ E
-      {{{ (n:nat) (z:Z), RET (#z, #n); Q z n }}}.
+      incr_counter1 c @ E
+      {{{ (n:nat) (z:nat), RET (#z, #n); Q z n }}}.
   Proof.
     iIntros (Hsubset Hpos Hineq Φ) "(#Hinv & #Hvs1 & #Hvs2 & HP) HΦ".
-    rewrite /incr_counter.
+    rewrite /incr_counter1.
     wp_pures.
     wp_bind (rand _)%E.
     iInv N as ">(%ε & %m & %l & %z & H1 & H2 & H3 & H4 & -> & H5 & H6)" "Hclose".
@@ -160,22 +225,24 @@ Section impl1.
     iInv N as ">(%ε & %m & % & %z & H1 & H2 & H3 & H4 & -> & H5 & H6)" "Hclose".
     wp_faa.
     iMod ("Hvs2" with "[$]") as "[H6 HQ]".
+    replace (#(z+n)) with (#(z+n)%nat); last first.
+    { by rewrite Nat2Z.inj_add. }
     iMod ("Hclose" with "[$H1 $H2 $H3 $H4 $H5 $H6]") as "_"; first done.
     iModIntro.
     wp_pures.
     by iApply "HΦ".
   Qed.
 
-  Lemma allocate_tape_spec N E c γ1 γ2 γ3:
+  Lemma allocate_tape_spec1 N E c γ1 γ2 γ3:
     ↑N ⊆ E->
-    {{{ inv N (counter_inv_pred c γ1 γ2 γ3) }}}
-      allocate_tape #() @ E
+    {{{ inv N (counter_inv_pred1 c γ1 γ2 γ3) }}}
+      allocate_tape1 #() @ E
       {{{ (v:val), RET v;
           ∃ (α:loc), ⌜v=#lbl:α⌝ ∗ α ◯↪N (3%nat; []) @ γ2
       }}}.
   Proof.
     iIntros (Hsubset Φ) "#Hinv HΦ".
-    rewrite /allocate_tape.
+    rewrite /allocate_tape1.
     wp_pures.
     wp_alloctape α as "Hα".
     iInv N as ">(%ε & %m & %l & %z & H1 & H2 & H3 & H4 & -> & H5 & H6)" "Hclose".
@@ -189,18 +256,18 @@ Section impl1.
     by iFrame.
   Qed.
 
-  Lemma incr_counter_tape_spec_some N E c γ1 γ2 γ3 (ε2:R -> nat -> R) (P: iProp Σ) (Q:Z->iProp Σ) (α:loc) (n:nat) ns:
+  Lemma incr_counter_tape_spec_some1 N E c γ1 γ2 γ3 (ε2:R -> nat -> R) (P: iProp Σ) (Q:nat->iProp Σ) (α:loc) (n:nat) ns:
     ↑N⊆E -> 
-    {{{ inv N (counter_inv_pred c γ1 γ2 γ3) ∗
-        □ (∀ (z:Z), P ∗ own γ3 (●F z) ={E∖↑N}=∗
-                          own γ3 (●F(z+n)%Z)∗ Q z) ∗
+    {{{ inv N (counter_inv_pred1 c γ1 γ2 γ3) ∗
+        □ (∀ (z:nat), P ∗ own γ3 (●F z) ={E∖↑N}=∗
+                          own γ3 (●F(z+n)%nat)∗ Q z) ∗
         P ∗ α ◯↪N (3%nat; n::ns) @ γ2
     }}}
-      incr_counter_tape c #lbl:α @ E
-      {{{ (z:Z), RET (#z, #n); Q z ∗ α ◯↪N (3%nat; ns) @ γ2}}}.
+      incr_counter_tape1 c #lbl:α @ E
+      {{{ (z:nat), RET (#z, #n); Q z ∗ α ◯↪N (3%nat; ns) @ γ2}}}.
   Proof.
     iIntros (Hsubset Φ) "(#Hinv & #Hvs & HP & Hα) HΦ".
-    rewrite /incr_counter_tape.
+    rewrite /incr_counter_tape1.
     wp_pures.
     wp_bind (rand(_) _)%E.
     iInv N as ">(%ε & %m & %l & %z & H1 & H2 & H3 & H4 & -> & H5 & H6)" "Hclose".
@@ -226,27 +293,29 @@ Section impl1.
     iInv N as ">(%ε & %m & % & %z & H1 & H2 & H3 & H4 & -> & H5 & H6)" "Hclose".
     wp_faa.
     iMod ("Hvs" with "[$]") as "[H6 HQ]".
+    replace (#(z+n)) with (#(z+n)%nat); last first.
+    { by rewrite Nat2Z.inj_add. }
     iMod ("Hclose" with "[$H1 $H2 $H3 $H4 $H5 $H6]") as "_"; first done.
     iModIntro. wp_pures.
     iApply "HΦ".
     by iFrame.
   Qed. 
     
-  Lemma incr_counter_tape_spec_none N E c γ1 γ2 γ3 (ε2:R -> nat -> R) (P: iProp Σ) (T: nat -> iProp Σ) (Q: Z -> nat -> iProp Σ)(α:loc) (ns:list nat):
+  Lemma incr_counter_tape_spec_none1 N E c γ1 γ2 γ3 (ε2:R -> nat -> R) (P: iProp Σ) (T: nat -> iProp Σ) (Q: nat -> nat -> iProp Σ)(α:loc) (ns:list nat):
     ↑N ⊆ E->
     (∀ ε n, 0<= ε -> 0<= ε2 ε n)%R->
     (∀ (ε:R), 0<=ε -> ((ε2 ε 0%nat) + (ε2 ε 1%nat)+ (ε2 ε 2%nat)+ (ε2 ε 3%nat))/4 <= ε)%R →
-    {{{ inv N (counter_inv_pred c γ1 γ2 γ3) ∗
+    {{{ inv N (counter_inv_pred1 c γ1 γ2 γ3) ∗
         □(∀ (ε:R) (n : nat), P ∗ ●↯ ε @ γ1 ={E∖↑N}=∗ (⌜(1<=ε2 ε n)%R⌝∨●↯ (ε2 ε n) @ γ1 ∗ T n) ) ∗
-        □ (∀ (n:nat) (z:Z), T n ∗ own γ3 (●F z) ={E∖↑N}=∗
-                          own γ3 (●F(z+n)%Z)∗ Q z n) ∗
+        □ (∀ (n:nat) (z:nat), T n ∗ own γ3 (●F z) ={E∖↑N}=∗
+                          own γ3 (●F(z+n)%nat)∗ Q z n) ∗
         P ∗ α ◯↪N (3%nat; []) @ γ2
     }}}
-      incr_counter_tape c #lbl:α @ E
-      {{{ (z:Z) (n:nat), RET (#z, #n); Q z n ∗ α ◯↪N (3%nat; []) @ γ2 }}}.
+      incr_counter_tape1 c #lbl:α @ E
+      {{{ (z:nat) (n:nat), RET (#z, #n); Q z n ∗ α ◯↪N (3%nat; []) @ γ2 }}}.
   Proof.
     iIntros (Hsubset Hpos Hineq Φ) "(#Hinv & #Hvs1 & #Hvs2 & HP & Hα) HΦ".
-    rewrite /incr_counter_tape.
+    rewrite /incr_counter_tape1.
     wp_pures.
     wp_bind (rand(_) _)%E.
     iInv N as ">(%ε & %m & %l & %z & H1 & H2 & H3 & H4 & -> & H5 & H6)" "Hclose".
@@ -270,6 +339,8 @@ Section impl1.
     iInv N as ">(%ε & %m & % & %z & H1 & H2 & H3 & H4 & -> & H5 & H6)" "Hclose".
     wp_faa.
     iMod ("Hvs2" with "[$]") as "[H6 HQ]".
+    replace (#(z+n)) with (#(z+n)%nat); last first.
+    { by rewrite Nat2Z.inj_add. }
     iMod ("Hclose" with "[$H1 $H2 $H3 $H4 $H5 $H6]") as "_"; first done.
     iModIntro.
     wp_pures.
@@ -277,15 +348,15 @@ Section impl1.
   Qed.
 
   
-  Lemma counter_presample NS (N : nat)  z E ns α
+  Lemma counter_presample_spec1 NS (N : nat)  z E ns α
      (ε2 : R -> nat -> R)
     (P : iProp Σ) (Q : val-> iProp Σ) T γ1 γ2 γ3 c:
     TCEq N (Z.to_nat z) →
     ↑NS ⊆ E ->
     (∀ ε n, 0<= ε -> 0<=ε2 ε n)%R ->
     (∀ (ε:R), 0<= ε ->SeriesC (λ n, if (bool_decide (n≤N)) then 1 / (S N) * ε2 ε n else 0%R)%R <= ε)%R->
-    inv NS (counter_inv_pred c γ1 γ2 γ3) -∗
-    (□∀ (ε:R) n, (P ∗ ●↯ ε @ γ1) ={E∖↑NS}=∗
+    inv NS (counter_inv_pred1 c γ1 γ2 γ3) -∗
+    (□∀ (ε:R) n, (P ∗ ●↯ ε@ γ1) ={E∖↑NS}=∗
         (⌜(1<=ε2 ε n)%R⌝ ∨(●↯ (ε2 ε n) @ γ1 ∗ T (n)))) 
         -∗
     P -∗ α ◯↪N (N; ns) @ γ2 -∗
@@ -340,19 +411,19 @@ Section impl1.
     iApply ("Hcnt" $! (state_upd_tapes <[α:= (Z.to_nat z; ns' ++[sample]):tape]> σ) with "[$]").
   Qed. 
 
-  Lemma read_counter_spec N E c γ1 γ2 γ3 P Q:
+  Lemma read_counter_spec1 N E c γ1 γ2 γ3 P Q:
     ↑N ⊆ E ->
-    {{{  inv N (counter_inv_pred c γ1 γ2 γ3) ∗
-        □ (∀ (z:Z), P ∗ own γ3 (●F z) ={E∖↑N}=∗
+    {{{  inv N (counter_inv_pred1 c γ1 γ2 γ3) ∗
+        □ (∀ (z:nat), P ∗ own γ3 (●F z) ={E∖↑N}=∗
                     own γ3 (●F z)∗ Q z)
          ∗ P
     }}}
-      read_counter c @ E
-      {{{ (n':Z), RET #n'; Q n'
+      read_counter1 c @ E
+      {{{ (n':nat), RET #n'; Q n'
       }}}.
   Proof.
     iIntros (Hsubset Φ) "(#Hinv & #Hvs & HP) HΦ".
-    rewrite /read_counter.
+    rewrite /read_counter1.
     wp_pure.
     iInv N as ">(%ε & %m & %l & %z & H1 & H2 & H3 & H4 & -> & H5 & H6)" "Hclose".
     wp_load.
@@ -363,3 +434,87 @@ Section impl1.
     
   
 End impl1.
+
+Program Definition random_counter1 `{!conerisGS Σ}: random_counter :=
+  {| new_counter := new_counter1;
+    incr_counter := incr_counter1;
+    allocate_tape:= allocate_tape1;
+    incr_counter_tape := incr_counter_tape1;
+    read_counter:=read_counter1;
+    counterG := counterG1;
+    error_name := gname;
+    tape_name := gname;
+    counter_name :=gname;
+    is_counter _ N c γ1 γ2 γ3 := inv N (counter_inv_pred1 c γ1 γ2 γ3);
+    counter_error_auth _ γ x := ●↯ x @ γ;
+    counter_error_frag _ γ x := ◯↯ x @ γ;
+    counter_tapes_auth _ γ m := (●m@γ)%I;
+    counter_tapes_frag _ γ α N ns := (α◯↪N (N;ns) @ γ)%I;
+    counter_content_auth _ γ z := own γ (●F z);
+    counter_content_frag _ γ f z := own γ (◯F{f} z);
+    new_counter_spec _ := new_counter_spec1;
+    incr_counter_spec _ := incr_counter_spec1;
+    allocate_tape_spec _ :=allocate_tape_spec1;
+    incr_counter_tape_spec_some _ :=incr_counter_tape_spec_some1;
+    incr_counter_tape_spec_none _ := incr_counter_tape_spec_none1;
+    counter_presample_spec _ :=counter_presample_spec1;
+    read_counter_spec _ :=read_counter_spec1
+  |}.
+Next Obligation.
+  simpl.
+  iIntros (??????) "(%&<-&H1)(%&<-&H2)".
+  iCombine "H1 H2" gives "%H". by rewrite excl_auth.excl_auth_auth_op_valid in H.
+Qed.
+Next Obligation.
+  simpl.
+  iIntros (??????) "(%&<-&H1)(%&<-&H2)".
+  iCombine "H1 H2" gives "%H". by rewrite excl_auth.excl_auth_frag_op_valid in H.
+Qed.
+Next Obligation.
+  simpl.
+  iIntros (??????) "H1 H2".
+  iApply (hocap_error_agree with "[$][$]").
+Qed.
+Next Obligation.
+  simpl. iIntros (???????) "??".
+  iApply (hocap_error_update with "[$][$]").
+Qed.
+Next Obligation.
+  simpl. 
+  iIntros (?????????) "H1 H2".
+  iDestruct (ghost_map_elem_frac_ne with "[$][$]") as "%"; last done.
+  rewrite dfrac_op_own dfrac_valid_own. apply Qp.not_add_le_r.
+Qed.
+Next Obligation.
+  simpl.
+  iIntros.
+  iApply (hocap_tapes_agree with "[$][$]").
+Qed.
+Next Obligation.
+  iIntros.
+  iApply (hocap_tapes_presample with "[$][$]").
+Qed.
+Next Obligation.
+  simpl.
+  iIntros (??????) "H1 H2".
+  iCombine "H1 H2" gives "%H". by rewrite auth_auth_op_valid in H.
+Qed.
+Next Obligation.
+  simpl. iIntros (???? z z' ?) "H1 H2".
+  iCombine "H1 H2" gives "%H".
+  apply frac_auth_included_total in H. iPureIntro.
+  by apply nat_included.
+Qed.
+Next Obligation.
+  simpl. iIntros (??????) "H1 H2".
+  iCombine "H1 H2" gives "%H".
+  iPureIntro.
+  by apply frac_auth_agree_L in H.
+Qed.
+Next Obligation.
+  simpl. iIntros (????????) "H1 H2".
+  iMod (own_update_2 _ _ _ (_ ⋅ _) with "[$][$]") as "[$$]"; last done.
+  apply frac_auth_update.
+  apply nat_local_update. lia.
+Qed.
+  
